% Preamble.
\documentclass[12pt]{article}
\usepackage[margin=1.25in]{geometry}
\usepackage[fleqn]{amsmath}
\usepackage{textcomp}
\usepackage{gensymb}
\usepackage{amsfonts}
\usepackage{enumitem}
%\usepackage{tikz}  % Include for figures.
%\usepackage{subfiles}  % Include for subfiles.

%% Title macros.
\newcommand{\HOMEWORKNUM}{26}
\newcommand{\NAME}{D. Choi}
\newcommand{\DATE}{2020-07-01}

\title{\vspace{-2\baselineskip}MATH 225 - Homework \#\HOMEWORKNUM}
\author{\NAME}
\date{\DATE}

%% Formatting options.
%\pagenumbering{gobble}  % Include for single-page document.


% Document.
\begin{document}
\maketitle

\section*{1.}
\textit{Verify that}
\begin{equation*}
	y = C_1 e^x + C_2 x e^x
\end{equation*}
\textit{is a solution to the differential equation}
\begin{equation*}
	y^{\prime\prime} - 2y^\prime + y = 0
	.
\end{equation*}
First, find $y^\prime$ and $y^{\prime\prime}$.
\begin{align*}
	y &= C_1 e^x + C_2 e^x x, \\
	y^\prime &= C_1 e^x + C_2 e^x x + C_2 e^x, \\
	y^{\prime\prime} &= C_1 e^x + C_2 e^x x + 2C_2 e^x.
\end{align*}
Substitute the right-hand sides into the equation.
\begin{gather*}
	0 \overset{?}{=}
	y^{\prime\prime} - 2y^\prime + y
	\\
	0 \overset{?}{=}
	(C_1 e^x + C_2 e^x x + 2C_2 e^x)
	- 2(C_1 e^x + C_2 e^x x + C_2 e^x)
	+ (C_1 e^x + C_2 e^x x)
	\\
	0 \overset{?}{=}
	(2 - 2)(C_1 e^x)
	+
	(2 - 2)(C_2 e^x x)
	+
	(2 - 2)(C_2 e^x)
	\\
	0 =
	0
	.
\end{gather*}

\section*{2.}
Verify the solution to the differential equation.
\begin{enumerate}[label=(\alph*)]
	\item
	\textit{Equation: $y^\prime = 2x$.}
	\textit{Solution: $y = x^2$.}
	\begin{equation*}
		y^\prime = \frac{d}{dx} y = \frac{d}{dx} x^2 = 2x.
	\end{equation*}
	\newpage
	
	\item
	\textit{Equation: $y^\prime + 3y = 6x + 11$.}
	\textit{Solution: $y = e^{-3x} + 2x + 3$.}
	\begin{equation*}
		y^\prime = -3e^{-3x} + 2.
	\end{equation*}
	Thus,
	\begin{gather*}
		6x + 11 \overset{?}{=} y^\prime + 3y \\
		6x + 11 \overset{?}{=} (-3e^{-3x} + 2) + 3(e^{-3x} + 2x + 3) \\
		6x + 11 \overset{?}{=} (3 - 3)(e^{-3x}) + 3(2x) + 3(3) + 2 \\
		6x + 11 = 6x + 11.
	\end{gather*}
	
	\item
	\textit{Equation: $y^{\prime\prime} - 3y^\prime + 2y = 24e^{-2x}$.}
	\textit{Solution: $y = 3e^x - 4e^{2x} + 2e^{-2x}$.}
	\begin{align*}
		y &= 3e^x - 4e^{2x} + 2e^{-2x}, \\
		y^\prime &= 3e^x - 8e^{2x} - 4e^{-2x}, \\
		y^{\prime\prime} &= 3e^x - 16e^{2x} + 8e^{-2x}.
	\end{align*}
	Thus,
	\begin{align*}
		24e^{-2x} &\overset{?}{=} y^{\prime\prime} - 3y^\prime + 2y \\
		24e^{-2x} &\overset{?}{=}
		(3e^x - 16e^{2x} + 8e^{-2x}) \\
		&\quad - 3(3e^x - 8e^{2x} - 4e^{-2x}) \\
		&\quad + 2(3e^x - 4e^{2x} + 2e^{-2x}) \\
		24e^{-2x} &\overset{?}{=}
		(3 - 9 + 6)(e^x) + (-16 + 24 - 8)(e^{2x}) + (8 + 12 + 4)(e^{-2x}) \\
		24e^{-2x} &= 24e^{2x}.
	\end{align*}
\end{enumerate}

\end{document}